All new benchmarks working. If conditionals now supported. Dafny verification extended to generate new kinds of invariants and pc to handle conditionals. New lemma generation added to handle conditionals. Emits in dafny wrapped in functions to support conditionals. Sketch parser bugs fixed.

compiler/src/casper/CasperScheduler.java
@@ -250,7 +250,7 @@ public class CasperScheduler extends JL7Scheduler {
      */
     public Goal ScaffoldGenerated (Job job)
     {
-		Goal g = internGoal(new VisitorGoal(job, new GenerateScaffold()));
+		Goal g = internGoal(new VisitorGoal(job, new GenerateScaffold(extInfo.nodeFactory())));
 		
     	try {
 			g.addPrerequisiteGoal(VerificationCodeGenerated(job), this);
